LeanFomega/Kinding/Substitute.lean
@@ -10,14 +10,29 @@ structure KindingSubst (σ : Subst Ty) (Δ1 Δ2 : List Kind) where
 
 notation:35 Γ:35 " -[" σ "]> " Δ:35 => KindingSubst σ Γ Δ
 
+theorem KindingSubst.id Δ : Δ -[+0]> Δ := sorry
+
 theorem KindingSubst.re (j : Δ2[y]? = some A) (m : Δ1 -[σ]> Δ2) : A::Δ1 -[re y::σ]> Δ2 := sorry
 
 theorem KindingSubst.su (j : Δ2 ⊢ₖ a : A) (m : Δ1 -[σ]> Δ2) : A::Δ1 -[su a::σ]> Δ2 := sorry
 
-theorem Kinding.comp : A -[σ]> B -> B -[τ]> C -> A -[σ ∘ τ]> C := sorry
+theorem KindingSubst.lift A :
+  Δ1 -[σ]> Δ2 ->
+  A::Δ1 -[σ.lift]> A::Δ2
+:= sorry
 
-theorem Kinding.subst (m : Δ1 -[σ]> Δ2) : Δ1 ⊢ₖ A : K -> Δ2 ⊢ₖ A[σ] : K := sorry
+theorem KindingSubst.comp : A -[σ]> B -> B -[τ]> C -> A -[σ ∘ τ]> C := sorry
 
-theorem Kinding.beta : (A::Δ) ⊢ₖ b : B -> Δ ⊢ₖ t : A -> Δ ⊢ₖ b[su t::+0] : B := sorry
+theorem KindingRen.to (m : A -⟨r⟩> B) : A -[r.to]> B := sorry
+
+theorem Kinding.subst (m : Δ1 -[σ]> Δ2) : Δ1 ⊢ₖ A : K -> Δ2 ⊢ₖ A[σ] : K
+| var h => m.act h
+| lam j => lam (j.subst $ m.lift _)
+| app j1 j2 => app (j1.subst m) (j2.subst m)
+| all j => all (j.subst $ m.lift _)
+| arrow j1 j2 => arrow (j1.subst m) (j2.subst m)
+
+theorem Kinding.beta : (A::Δ) ⊢ₖ b : B -> Δ ⊢ₖ t : A -> Δ ⊢ₖ b[su t::+0] : B
+| j1, j2 => subst (.su j2 $ .id _) j1
 
 end LeanFomega
